examples/fibo.v
@@ -20,15 +20,13 @@
 
 Require Import Coq.Program.Wf.
 Require Import Coq.Strings.Ascii.
-Require Import Coq.Strings.String.
-Require Import FreeSpec.Exec.Plugin.
 Require Import FreeSpec.Stdlib.Console.
 Require Import FreeSpec.Program.
-Require Import FreeSpec.Compose.
 Require Import Prelude.Control.
 
 Local Open Scope prelude_scope.
 Local Open Scope char_scope.
+
 Require Import PeanoNat.
 
 Definition ascii_of_nat n :=
