examples/hello.v
@@ -18,11 +18,8 @@
  * along with this program. If not, see <http://www.gnu.org/licenses/>.
  *)
 
-Require Import Coq.Strings.String.
-Require Import FreeSpec.Exec.Plugin.
 Require Import FreeSpec.Stdlib.Console.
 Require Import FreeSpec.Program.
-Require Import FreeSpec.Compose.
 Require Import Prelude.Control.
 
 Local Open Scope prelude_scope.
