stdlib/console/demos/Hello.v
@@ -19,10 +19,8 @@
  * along with this program. If not, see <http://www.gnu.org/licenses/>.
  *)
 
-Require Import Coq.Strings.String.
 Require Import FreeSpec.Stdlib.Console.
 Require Import FreeSpec.Program.
-Require Import FreeSpec.Compose.
 Require Import Prelude.Control.
 
 Local Open Scope prelude_scope.
@@ -31,4 +29,3 @@ Definition hello {ix} `{Use Console.i ix} : Program ix unit :=
   Console.echo "Hello, world".
 
 Exec hello.
-
