stdlib/console/theories/Console.v
@@ -18,10 +18,9 @@
  * along with this program. If not, see <http://www.gnu.org/licenses/>.
  *)
 
-Require Import FreeSpec.Exec.Plugin.
-Require Import Coq.Strings.String.
+Require Import FreeSpec.Exec.
+Require Export Coq.Strings.String.
 Require Import FreeSpec.Program.
-Require Import FreeSpec.Compose.
 
 Module Console.
   Inductive i: Type -> Type :=
